removed old (deprecated) Appraisal files

src/Appraisal.v
@@ -1,22 +1,38 @@
-Require Import GenStMonad MonadVM MonadAM ConcreteEvidence.
+Require Import GenStMonad MonadVM MonadAM ConcreteEvidence MonadVMFacts.
 Require Import StAM VM_IO_Axioms Maps VmSemantics Event_system Term_system.
 
 Require Import Coq.Arith.Peano_dec.
 
+Require Import StructTactics.
+
+Require Import Coq.Program.Tactics Coq.Program.Equality.
 
 Require Import List.
 Import ListNotations.
 
-Check map_get.
+Set Nested Proofs Allowed.
 
-Inductive evidenceEvent: Ev -> Prop :=
-| uev: forall n p i args, evidenceEvent (umeas n p i args)
-| sev: forall n p, evidenceEvent (sign n p)
-| hev: forall n p, evidenceEvent (hash n p).
+Definition extractSig (e:EvidenceC) : VM (BS * EvidenceC) :=
+  match e with
+  | ggc bs e' => ret (bs, e')
+  | _ => failm
+  end.
 
-Definition ioEvent (t:AnnoTerm) (p:Plc) (ev:Ev) : Prop :=
-  let es := ev_sys t p in
-  ev_in ev es /\ evidenceEvent ev.
+(*
+Definition extractHsh (e:EvidenceC) : VM (BS * EvidenceC) :=
+  match e with
+  | hhc bs e' => ret (bs, e')
+  | _ => failm
+  end. *)
+
+(*
+Definition extractComp (e:EvidenceC) : VM (EvidenceC * EvidenceC) :=
+  match e with
+  | ssc e1 e2 => ret (e1,e2)
+  | ppc e1 e2 => ret (e1,e2)
+  | _ => failm
+  end.
+*)
 
 Definition am_get_app_asp (p:Plc) (i:ASP_ID) : AM ASP_ID :=
   m <- gets st_aspmap ;;
@@ -26,196 +42,3151 @@ Definition am_get_app_asp (p:Plc) (i:ASP_ID) : AM ASP_ID :=
   | None => failm
   end.
 
-Fixpoint gen_appraisal_term (et:Evidence) : AM Term :=
-  match et with
-  | mt => ret (asp CPY)
-  | uu i_t p e'_t =>
-    app_id <- am_get_app_asp p i_t ;;
-    let t1 := (asp (ASPC app_id [])) in
-    t2 <- gen_appraisal_term e'_t ;;
-    ret (bpar (NONE,NONE) t1 t2)
-  | ss e1 e2 =>
-    t1 <- gen_appraisal_term e1 ;;
-    t2 <- gen_appraisal_term e2 ;;
-    ret (bpar (NONE,NONE) t1 t2)
-  | _ => ret (asp CPY)
+Definition am_get_sig_asp (p:Plc) : AM ASP_ID :=
+  m <- gets st_sigmap ;;
+  let maybeId := map_get m p in
+  match maybeId with
+  | Some i' => ret i'
+  | None => failm
   end.
 
-Definition at1 := (asp (ASPC 1 [])).
-Definition at2 := (asp (ASPC 2 [])).
-Definition aterm := bseq (NONE,NONE) at1 at2.
+Definition test_phrase_match (t:Term) : nat :=
+  match t with
+  | lseq t (asp SIG) => 3
+  | _ => 3
+  end.
 
-Definition aet := eval aterm 0 mt.
-Print aet.
-Compute aet.
+Definition invokeUSM' (x:nat) (i:ASP_ID) (l:list Arg) : VM EvidenceC :=
+  e <- get_ev ;;
+  p <- get_pl ;;
+  add_tracem [Term.umeas x p i l];;
+  ret (uuc i x e).
 
-Definition acomp := (gen_appraisal_term aet).
+Definition checkSig (x:nat) (i:ASP_ID) (l:list Arg) : VM BS :=
+  (*p <- get_pl ;; *)
+  add_tracem [Term.umeas x 0 i l];;
+  ret 78.
 
-Check runSt.
+Print EvidenceC.
 
-Definition ast :=
-  mkAM_St [] 0 [((0,1),33); ((0,2),44)].
+Definition extractUev (e:EvidenceC) : VM (BS * EvidenceC) :=
+  match e with
+  | uuc i bs e' => ret (bs,e')
+  | _ => failm
+  end.
 
-Definition appterm := (runSt ast acomp).
-Compute appterm.
+
+Definition checkUSM (x:nat) (i:ASP_ID) (l:list Arg) (bs:BS) : VM BS :=
+  (* p <- get_pl ;; *)
+  add_tracem [Term.umeas x 0 i ([bs] ++ l)] ;;
+  ret 56.
+
+Compute (eval (lseq (asp (ASPC 42 [42;42])) (asp (ASPC 43 [43;43]))) 0 (uu 1 [2;3] 0 mt)).
+
+Compute (eval (lseq (asp (ASPC 43 [43;43])) (asp (ASPC 42 [42;42]))) 0 (uu 1 [2;3] 0 mt)).
+
 (*
-     = (Some
-          (bpar (NONE, NONE) (bpar (NONE, NONE) (asp (ASPC 3 [])) (asp CPY))
-             (bpar (NONE, NONE) (asp (ASPC 4 [])) (asp CPY))),
-       {| am_nonceMap := []; am_nonceId := 0; st_aspmap := [(0, 1, 3); (0, 2, 4)] |})
-     : option Term * AM_St
+Compute (eval (bseq (ALL,NONE) (asp (ASPC 1 [1;1])) (asp (ASPC 2 [2;2]))) 0 (uu 1 [2;3] 0 mt)).
 *)
 
-Compute aet.
+
+Fixpoint build_app_comp (t:AnnoTerm) (p:Plc) : AM (VM (EvidenceC -> EvidenceC)) :=
+  match t with
+  | alseq (n,n') t' (aasp r' SIG) =>
+    app_id <- am_get_sig_asp p ;;
+    d <- build_app_comp t' p ;;
+    let c :=
+        (
+        e <- get_ev ;;
+        pr <- extractSig e ;;
+        let '(bs,e') := pr in
+        res <- checkSig n app_id ([encodeEv e'] ++ [bs] (* ++ args*) ) ;;
+        put_ev e' ;;
+        e_res <- d ;;
+        ret (fun x => ggc res (e_res x))) in
+    ret c   
+
+  | alseq (n,n') t1 t2 =>
+    c <- build_app_comp t1 p ;;
+    d <- build_app_comp t2 p ;;
+    let cc :=
+        (
+          g <- d ;;
+          f <- c ;;
+          ret (fun x => g (f x))
+          (*
+        e <- get_ev ;;
+        pr <- extractComp e ;;
+        let '(e1,e2) := pr in
+        put_ev e1 ;;
+        e1_res <- c ;;
+        put_ev e2 ;;
+        e2_res <- d ;;
+        ret (ssc e1_res e2_res)*)) in
+    ret cc
+
+        
+  | aasp (n,n') (ASPC i args) =>
+    app_id <- am_get_app_asp p i ;;
+    let c :=
+        (
+        e <- get_ev ;;
+        pr <- extractUev e ;;
+        let '(bs,e') := pr in
+        res <- checkUSM n app_id args bs ;;
+        put_ev e' ;;
+        ret (fun x => (uuc n res x) )) in
+    ret c
+
+  | aasp (n,n') (SIG) =>
+    app_id <- am_get_sig_asp p ;;
+    let c :=
+        e <- get_ev ;;
+        pr <- extractSig e ;;
+        let '(bs,e') := pr in
+        res <- checkSig n app_id ([encodeEv e'] ++ [bs] (* ++ args*) ) ;;
+        put_ev e' ;;
+        ret (fun x => ggc res x) in
+        
+    ret c
+        
 (*
-     = ss (uu 1 0 mt) (uu 2 0 mt)
-     : Evidence
- *)
-Definition evc := (run_vm (annotated aterm) empty_vmst).
-Compute evc.
+  | aasp (n,n') (HSH) =>
+   (* app_id <- am_get_sig_asp p ;; *) (* TODO: get_hsh_asp impl *) 
+    let c :=
+        e <- get_ev ;;
+        pr <- extractHsh e ;;
+        let '(bs,e') := pr in
+        (*
+        res <- checkSig n app_id ([encodeEv e'] ++ [bs] (* ++ args*) ) ;;
+        put_ev e' ;; (* TODO: does this have any effect? *) 
+        ret (ggc res e') *)
+        put_ev e' ;;
+        ret (fun x => hhc 0 x) in
+        
+    ret c     *)
+        
 
-Fixpoint moveEv (e:EvidenceC) : (EvidenceC * BS) :=
-  match e with
-  | mtc => (mtc, 0)
-  | uuc i bs e' => (e',bs)
-  | ggc bs e' => (e',bs)
-  | hhc bs e' => (e',bs)
-  | nnc n bs e' => (e',bs)
-  | ssc mtc e2 => moveEv e2
-  | ssc e1 e2 => let (e1',bs) := moveEv e1 in
-                ((ssc e1' e2),bs)
-  | ppc e1 e2 => let (e1',bs) := moveEv e1 in
-                ((ppc e1' e2),bs)
-  end.
-
-Compute (moveEv (st_ev evc)).
+  | aasp (n,n') (CPY) =>
     
-
-Definition getBS : VM BS :=
-  e <- gets st_ev ;;
-  let (e',bs) := moveEv e in
-  put_ev e' ;;
-  ret bs.
-  
-Definition do_prim_app (x:nat) (p:Plc) (a:ASP) : VM EvidenceC :=
-  e <- gets st_ev ;;
-  bs <- getBS ;;
-  let args := [bs] in
-  match a with
-  | CPY => copyEv x p
-  | ASPC asp_id _ =>
-    invokeUSM x asp_id p args
-  | SIG => signEv x p
-  | HSH => hashEv x p
+    (*p <- gets am_pl ;; *)
+   (* app_id <- am_get_sig_asp p ;; *) (* TODO: get_hsh_asp impl *) 
+    let c :=
+        (*e <- get_ev ;; *)
+        (*
+        pr <- extractHsh e ;;
+        let '(bs,e') := pr in
+        (*
+        res <- checkSig n app_id ([encodeEv e'] ++ [bs] (* ++ args*) ) ;;
+        put_ev e' ;; (* TODO: does this have any effect? *) 
+        ret (ggc res e') *)
+        put_ev e' ;;
+        ret (hhc 0 mtc) *)
+        ret (fun x => x) in
+        
+    ret c
+        
+  | aatt r q t' =>
+    (*modify_plc q ;; *)
+    build_app_comp t' q
+  (*| _ => ret (ret (fun _ => mtc)) *)
   end.
 
-Fixpoint build_comp_app (t:AnnoTerm): VM unit :=
-  match t with   
-  | aasp (n,_) a =>
-    p <- get_pl ;;
-    e <- do_prim_app n p a ;;
-    put_ev e
-  | alseq r t1 t2 =>
-    build_comp_app t1 ;;
-    build_comp_app t2
-  | abpar r _ t1 t2 =>
-    build_comp_app t1 ;;
-    build_comp_app t2
-  | _ => ret tt
-  end.
-
+(*
 Definition fromOpt{A:Type} (o:option A) (a:A) : A :=
   match o with
   | Some t => t
   | None => a
   end.
 
-Definition app_term := fromOpt (fst appterm) (asp CPY).
-Compute app_term.
+Definition run_app_comp (t:AnnoTerm) (p:Plc) (a_st:AM_St) (e_in:EvidenceC) : (EvidenceC -> EvidenceC) :=
+  let acomp := build_app_comp t p in (* AM (VM (EvidenceC -> EvidenceC)) *)
+  let vcomp_opt := runSt a_st acomp in (* (option (VM (EvidenceC -> EvidenceC)) * AM_St) *)
+  let vcomp := fromOpt (fst vcomp_opt) (ret (fun _ => mtc)) in (* (VM (EvidenceC -> EvidenceC)) *)
+  let vres_opt := runSt (mk_st e_in [] 0 []) vcomp in (* (option (EvidenceC -> EvidenceC) * VM_St) *)
+  fromOpt (fst vres_opt) ((fun _ => mtc)).
 
-Definition app_term' :=
-  (bpar (NONE, NONE) (asp (ASPC 44 [])) (asp CPY)).
+Definition run_app_comp' (t:AnnoTerm) (p:Plc) (st:AM_St) (e_in:EvidenceC) : ((option (EvidenceC -> EvidenceC)) * vm_st) :=
+  let acomp := build_app_comp t p in (* AM (VM (EvidenceC -> EvidenceC)) *)
+  let vcomp_opt := runSt st acomp in (* (option (VM (EvidenceC -> EvidenceC)) * AM_St) *)
+  let vcomp := fromOpt (fst vcomp_opt) (ret (fun _ => mtc)) in (* (VM (EvidenceC -> EvidenceC)) *)
+  let vres_opt := runSt (mk_st e_in [] 0 []) vcomp in
+  vres_opt.
 
-Definition app_term'' :=
-  (bpar (NONE, NONE) (asp (ASPC 33 [])) (asp (ASPC 44 [])) ).
+
+Definition at1 := (asp (ASPC 11 [])).
+(*Definition at2 := (asp (ASPC 22 [])). *)
+Definition term := lseq at1 (asp SIG).
+Definition aterm := annotated term.
+Compute aterm.
+
+Check run_vm.
+
+Definition aterm_vm_st := run_vm aterm empty_vmst.
+Compute aterm_vm_st.
+Definition aterm_ev := st_ev aterm_vm_st.
+Compute aterm_ev.
+
+Definition ast :=
+  mkAM_St [] 0 [((0,11),34); ((0,22),45)] [(0,42)].
+
+Compute run_app_comp' aterm 0 ast aterm_ev.
+
+Compute run_app_comp aterm 0 ast aterm_ev.
+*)
 
 
-Definition app_comp := (build_comp_app (annotated (app_term))).
+Inductive evMapped : Evidence -> AM_St -> Prop :=
+| evMappedMt : forall m, evMapped mt m
+| evMappedU : forall p i args e' m st,
+    m = st_aspmap st ->
+    evMapped e' st -> 
+    (exists j, bound_to m (p,i) j) -> 
+    evMapped (uu i args p e') st
+| evMappedG : forall e' m p st,
+    m = st_sigmap st ->
+    evMapped e' st ->
+    (exists j, bound_to m p j) ->
+    evMapped (gg p e') st
+(*| evMappedH : forall e' p st,
+    (*m = st_sigmap st -> *)
+    evMapped e' st ->
+    evMapped (hh p e') st *)
 
-Compute (st_ev evc).
+(*
+            
+| evMappedN : forall e' m nid st,
+    m = st_aspmap st ->
+    evMapped e' st ->
+    evMapped (nn nid e') st 
+| evMappedS : forall e1 e2 st,
+    evMapped e1 st ->
+    evMapped e2 st ->
+    evMapped (ss e1 e2) st
+| evMappedP : forall e1 e2 st,
+    evMapped e1 st ->
+    evMapped e2 st ->
+    evMapped (pp e1 e2) st *).
+Print eval.
+Print eval_asp.
 
-Definition newst := mk_st (st_ev evc) [] 0 [].
 
-Compute (runSt newst app_comp).
+Inductive allMapped : AnnoTerm -> AM_St -> Plc -> Evidence -> Prop :=
+| allMapped_cpy : forall r p st e,
+    (*m = st_aspmap st -> *)
+    (*p = am_pl st -> *)
+    evMapped e st ->
+    allMapped (aasp r (CPY)) st p e
+| allMapped_asp : forall m st p i r args e,
+    (*p = am_pl st -> *)
+    evMapped e st ->
+    m = st_aspmap st ->
+    (exists j, bound_to m (p,i) j) ->
+    allMapped (aasp r (ASPC i args)) st p e
+| allMapped_sig : forall r p st m e,
+    evMapped e st ->
+    (*p = am_pl st -> *)
+    m = st_sigmap st ->
+    (exists j, bound_to m p j) ->
+    allMapped (aasp r (SIG)) st p e
+(*| allMapped_hsh : forall r p st e,
+    evMapped e st ->
+    (*p = am_pl st -> *)
+    allMapped (aasp r (HSH)) st p e *)
+| allMapped_at : forall t' p q r st e m x y z z',
+    m = st_aspmap st ->
+    (*evMapped e m -> *) (* TODO: need this? *)
+    st = (mkAM_St x y z z') ->
+    allMapped t' (mkAM_St x y z z') q e ->
+    allMapped (aatt r q t') st p e
+| allMapped_lseq : forall t1 t2 p st r e,
+    (* m = st_aspmap st ->
+       evMapped e m -> *)  (* TODO: need this? *)
+    (*p = am_pl st -> *)
+    allMapped t1 st p e ->
+    allMapped t2 st p mt (*(eval (unanno t1) p e)*) -> (* TODO: is mt ok here? *)
+    allMapped (alseq r t1 t2) st p e
+(*| allMapped_bseq_nn : forall t1 t2 p st e r,
+    (*p = am_pl st -> *)
+    allMapped t1 st p mt ->
+    allMapped t2 st p mt ->
+    allMapped (abseq r (NONE,NONE) t1 t2) st p e
+| allMapped_bseq_na : forall t1 t2 p st e r,
+    (*p = am_pl st -> *)
+    allMapped t1 st p mt ->
+    allMapped t2 st p e ->
+    allMapped (abseq r (NONE,ALL) t1 t2) st p e
+| allMapped_bseq_an : forall t1 t2 p st e r,
+    (*p = am_pl st -> *)
+    allMapped t1 st p e ->
+    allMapped t2 st p mt ->
+    allMapped (abseq r (ALL,NONE) t1 t2) st p e
+| allMapped_bseq_aa : forall t1 t2 p st e r,
+    (*p = am_pl st -> *)
+    allMapped t1 st p e ->
+    allMapped t2 st p e ->
+    allMapped (abseq r (ALL,ALL) t1 t2) st p e
+| allMapped_bpar_nn : forall t1 t2 p st e r,
+    (*p = am_pl st -> *)
+    allMapped t1 st p mt ->
+    allMapped t2 st p mt ->
+    allMapped (abpar r (NONE,NONE) t1 t2) st p e
+| allMapped_bpar_na : forall t1 t2 p st e r,
+    (*p = am_pl st -> *)
+    allMapped t1 st p mt ->
+    allMapped t2 st p e ->
+    allMapped (abpar r (NONE,ALL) t1 t2) st p e
+| allMapped_bpar_an : forall t1 t2 p st e r,
+   (* p = am_pl st -> *)
+    allMapped t1 st p e ->
+    allMapped t2 st p mt ->
+    allMapped (abpar r (ALL,NONE) t1 t2) st p e
+| allMapped_bpar_aa : forall t1 t2 p st e r,
+    (*p = am_pl st ->*)
+    allMapped t1 st p e ->
+    allMapped t2 st p e ->
+    allMapped (abpar r (ALL,ALL) t1 t2) st p e*).
+
+(*
+Definition allMapped (t:AnnoTerm) (a_st:AM_St) (p:Plc) (e:Evidence) : Prop :=
+  evMapped (eval (unanno t) p e) a_st.
+*)
+
+Ltac debound :=
+  match goal with
+  | [H: bound_to _ _ _ |- _] => invc H
+  end.
+
+Ltac evMappedFacts :=
+  match goal with
+  | [H: evMapped (uu _ _ _ _) _ |- _] => invc H
+  | [H: evMapped (gg _ _) _ |- _] => invc H
+ (* | [H: evMapped (hh _ _) _ |- _] => invc H *)
+                                        (*
+  | [H: evMapped (nn _ _) _ |- _] => invc H
+  | [H: evMapped (ss _ _) _ |- _] => invc H
+  | [H: evMapped (pp _ _) _ |- _] => invc H  *)
+  end;
+  destruct_conjs;
+  try debound.
+
+Ltac allMappedFacts :=
+  (*
+  unfold allMapped in *;
+  df;
+  try evMappedFacts. *)
+
   
+  match goal with
+  | [H: allMapped (aasp _ _) _ _ _ |- _] => invc H
+  | [H: allMapped (aatt _ _ _) _ _ _ |- _] => invc H
+  | [H: allMapped (alseq _ _ _) _ _ _ |- _] => invc H
+ (* | [H: allMapped (abseq _ _ _ _) _ _ _ |- _] => invc H
+  | [H: allMapped (abpar _ _ _ _) _ _ _ |- _] => invc H *)
+  end;
+  destruct_conjs.
 
-Fixpoint build_comp (t:AnnoTerm): VM unit :=
-  match t with
-    
-  | aasp (n,_) a =>
-    p <- get_pl ;;
-    e <- do_prim n p a ;;
-    put_ev e
-  | aatt (reqi,rpyi) q t' =>
-    sendReq reqi q t' ;;
-    e <- get_ev ;;
-    doRemote t' q e rpyi ;;
-    e' <- receiveResp rpyi q ;;
-    put_ev e'
-  | alseq r t1 t2 =>
-    build_comp t1 ;;
-    build_comp t2 (* TODO: does evidence work out ok? *)
-  | abseq (x,y) (sp1,sp2) t1 t2 =>
-    e <- get_ev ;;
-    p <- get_pl ;;
-    pr <- split_evm x sp1 sp2 e p ;;
-    let '(e1,e2) := pr in
-    put_ev e1 ;;
-    build_comp t1 ;;
-    e1r <- get_ev ;;
-    put_ev e2 ;;
-    build_comp t2 ;;
-    e2r <- get_ev ;;
-    put_ev (ssc e1r e2r) ;;
-    add_tracem [Term.join (Nat.pred y) p]
-        
+
+
+Lemma allMappedAt : forall r n a p st e (*x y z z'*),
+    (*st = mkAM_St x y z z'-> *)
+    allMapped (aatt r n a) st p e ->
+    allMapped a (*(mkAM_St x y z z')*) st n e.
+Proof.
+  intros.
+  allMappedFacts.
+  df.
+  eauto.
+Defined.
+
 (*
 
-  | abseq (x,y) (sp1,sp2) t1 t2 =>
-    e <- get_ev ;;
-    p <- get_pl ;;
-    pr <- split_evm x sp1 sp2 e p ;;
-    let '(e1,e2) := pr in
-    put_ev e1 ;;
-    push_stackm e2 ;;
-    build_comp t1 ;;
-    e <- get_ev ;;
-    er <- pop_stackm ;; (* TODO:  is stack still necessary? *)
-    put_ev er ;;
-    push_stackm e ;;
-    build_comp t2 ;;
-    er' <- pop_stackm ;;
-    er'' <- get_ev ;;
-    put_ev (ssc er' er'') ;;
-    add_tracem [Term.join (Nat.pred y) p]
-*)
-  | abpar (x,y) (sp1,sp2) t1 t2 =>
-    e <- get_ev ;;
-    p <- get_pl ;;
-    pr <- split_evm x sp1 sp2 e p ;;
-    let '(e1,e2) := pr in
-    let res1 := parallel_att_vm_thread t1 e in
-    (* TODO: change this to a monadic function that consults an environment that is aware of the presence (or absence) of parallel avm threads.  Put initial evidence in store, let environment run the parallel thread and place result evidence, then query for result evidence here. *)
-    let res2 := parallel_att_vm_thread t2 e2 in
-    let el1 := parallel_vm_events t1 p in
-    let el2 := parallel_vm_events t2 p in
-    let loc1 := fst (range t1) in
-    let loc2 := fst (range t2) in
-    put_store loc1 res1 ;;
-    put_store loc2 res2 ;;
-    add_tracem (shuffled_events el1 el2) ;;
-    e1r <- get_store_at loc1 ;;
-    e2r <- get_store_at loc2 ;;
-    put_ev (ppc e1r e2r) ;;
-    add_tracem [Term.join (Nat.pred y) p]
+  unfold allMapped in *.
+  df.
+  eassumption.
+Defined. *)
+
+Ltac df :=
+  repeat (
+      cbn in *;
+      unfold runSt in *;
+      repeat break_let;
+      repeat (monad_unfold; cbn in *; find_inversion);
+      monad_unfold;
+      repeat dunit;
+      unfold snd in * ).
+
+Ltac dosome :=
+  repeat (
+      match goal with
+      | [H: match ?o with
+            | Some _ => _
+            | _ => _
+            end
+            =
+            (Some _, _) |- _] =>
+        destruct o; try solve_by_inversion
+      end; df).
+
+Ltac tacc H :=
+  (symmetry;
+   erewrite <- pl_immut in *;
+   rewrite H;
+   eauto ).
+
+Ltac ff := repeat break_match; try solve_by_inversion; df.
+
+Ltac dosome_eq y :=
+  match goal with
+  | [H: match ?x with _ => _ end = (Some _, _)  |- _] =>
+    destruct x eqn:y; try solve_by_inversion
   end.
+Ltac do_pair :=
+  match goal with
+  | [H: (_,_) = (Some _,_) |- _] => invc H
+  | [H: (Some _,_) = (_,_) |- _] => invc H
+  end.
+
+Ltac amsts :=
+  repeat match goal with
+         | H:vm_st |- _ => destruct H
+         end.
+
+Ltac dosome_eqj :=
+  let y := fresh in 
+  match goal with
+  | [H: match ?x with _ => _ end = (Some _, _)  |- _] =>
+    destruct x eqn:y; try solve_by_inversion
+  end.
+
+Ltac dosome'' :=
+  match goal with
+  | [H: (_,_) = (Some _, _) |- _] => invc H
+  end.
+
+Ltac domap :=
+  let n := fresh in
+  match goal with
+  | [H: match ?X with _ => _ end _ = (Some _, _) |- _] =>
+    destruct X eqn:n; try solve_by_inversion
+  end.
+
+
+Ltac doit' := repeat dosome_eqj;
+              repeat break_let;
+              repeat do_pair;
+              repeat break_let;
+              repeat do_pair;
+              repeat dosome''.
+
+Ltac doit := repeat doit'.
+
+
+
+(*
+  Ltac map_get_subst :=
+  match goal with
+  | [H: map_get ?A ?B = _,
+  H2: context[map_get ?A ?B] |- _] =>
+  rewrite H in *; clear H
+  end.
+ *)
+
+
+
+Ltac subst' :=
+  match goal with
+  | [H: ?A = _,
+        H2: context[?A] |- _] =>
+    rewrite H in *; clear H
+  | [H: ?A = _ |- context[?A]] =>
+    rewrite H in *; clear H
+  end.
+
+Ltac evShapeFacts :=
+  match goal with
+  | [H: Ev_Shape mtc _ |- _] => invc H
+  | [H: Ev_Shape _ mt |- _] => invc H
+  | [H: Ev_Shape (uuc _ _ _) _ |- _] => invc H
+  | [H: Ev_Shape _ (uu _ _ _ _) |- _] => invc H
+  | [H: Ev_Shape (ggc _ _) _ |- _] => invc H
+  | [H: Ev_Shape _ (gg _ _) |- _] => invc H
+  (*| [H: Ev_Shape (hhc _ _) _ |- _] => invc H
+  | [H: Ev_Shape _ (hh _ _) |- _] => invc H *)
+                                        (*
+  | [H: Ev_Shape (nnc _ _ _) _ |- _] => invc H
+  | [H: Ev_Shape _ (nn _ _) |- _] => invc H
+  | [H: Ev_Shape (ssc _ _) _ |- _] => invc H
+  | [H: Ev_Shape _ (ss _ _) |- _] => invc H
+  | [H: Ev_Shape (ppc _ _) _ |- _] => invc H
+  | [H: Ev_Shape _ (pp _ _) |- _] => invc H *)
+  end.
+
+Ltac haaa :=
+  let x:= fresh in
+  match goal with
+  | [H: context[match ?ee with | Some _ => _ | _ => _ end] |- _] =>
+    destruct ee eqn:x;
+    try solve_by_inversion
+  end; df; eauto.
+
+Ltac stt :=
+  cbn in *;
+  monad_unfold;
+  try solve_by_inversion;
+  repeat break_let;
+  dosome;
+  try haaa.
+
+
+
+
+(*
+Definition run_app_comp (t:AnnoTerm) (p:Plc) (a_st:AM_St) (e_in:EvidenceC) : (EvidenceC -> EvidenceC) :=
+  let acomp := build_app_comp t p in (* AM (VM (EvidenceC -> EvidenceC)) *)
+  let vcomp_opt := runSt a_st acomp in (* (option (VM (EvidenceC -> EvidenceC)) * AM_St) *)
+  let vcomp := fromOpt (fst vcomp_opt) (ret (fun _ => mtc)) in (* (VM (EvidenceC -> EvidenceC)) *)
+  let vres_opt := runSt (mk_st e_in [] 0 []) vcomp in (* (option (EvidenceC -> EvidenceC) * VM_St) *)
+  fromOpt (fst vres_opt) ((fun _ => mtc)).
+
+Definition run_app_comp' (t:AnnoTerm) (p:Plc) (st:AM_St) (e_in:EvidenceC) : ((option (EvidenceC -> EvidenceC)) * vm_st) :=
+  let acomp := build_app_comp t p in (* AM (VM (EvidenceC -> EvidenceC)) *)
+  let vcomp_opt := runSt st acomp in (* (option (VM (EvidenceC -> EvidenceC)) * AM_St) *)
+  let vcomp := fromOpt (fst vcomp_opt) (ret (fun _ => mtc)) in (* (VM (EvidenceC -> EvidenceC)) *)
+  let vres_opt := runSt (mk_st e_in [] 0 []) vcomp in
+  vres_opt.
+*)
+
+Ltac subst'' :=
+  match goal with
+  | H:?A = _, H2:context [ ?A ] |- _ => rewrite H in *
+  | H:?A = _ |- context [ ?A ] => rewrite H in *
+  end.
+Check build_app_comp.
+Lemma ba_const : forall a a_st a_st' o p,
+    build_app_comp a p a_st = (o, a_st') ->
+    a_st = a_st'.
+  (*
+    am_nonceMap a_st = am_nonceMap a_st' /\
+    am_nonceId a_st = am_nonceId a_st' /\
+    st_aspmap a_st = st_aspmap a_st' /\
+    st_sigmap a_st = st_sigmap a_st'. *)
+Proof.
+  intros.
+  generalizeEverythingElse a.
+  induction a; intros.
+  -
+    destruct a;
+      repeat (ff; eauto).
+  -
+    eauto.
+    (*
+    edestruct IHa.
+    eassumption.
+    destruct_conjs.
+    simpl in *.
+    subst.
+    tauto. *)
+  -
+    
+    df.
+    subst.
+    destruct a2.
+    +
+      destruct a;
+        repeat (ff;eauto).
+      
+    + (* aatt case *)
+      doit.
+      specialize IHa1 with (a_st:=a_st) (a_st':=a) (o:=o0) (p:=p).
+      concludes.
+      destruct_conjs.
+      specialize IHa2 with (a_st := a) (a_st':=a0) (o:=o1) (p:=p).
+      concludes.
+      subst.
+      
+      ff; eauto.
+
+    + (* alseq case *)
+
+      doit.
+      specialize IHa1 with (a_st:=a_st) (a_st':=a) (o:=o0) (p:=p).
+      concludes.
+      destruct_conjs.
+      specialize IHa2 with (a_st := a) (a_st':=a0) (o:=o1) (p:=p).
+      concludes.
+      subst.
+      ff; eauto.
+
+       (*
+    +
+            destruct (build_app_comp a1 p a_st) eqn:hey;
+         try solve_by_inversion.
+       destruct (build_app_comp (abseq r s a2_1 a2_2) p a) eqn:hi;
+         try solve_by_inversion.
+       specialize IHa1 with (a_st:=a_st) (a_st':=a) (o:=o0) (p:=p).
+       concludes.
+       destruct_conjs.
+       specialize IHa2 with (a_st := a) (a_st':=a0) (o:=o1) (p:=p).
+       concludes.
+       subst.
+       ff; eauto.
+    +
+                  destruct (build_app_comp a1 p a_st) eqn:hey;
+         try solve_by_inversion.
+       destruct (build_app_comp (abpar r s a2_1 a2_2) p a) eqn:hi;
+         try solve_by_inversion.
+       specialize IHa1 with (a_st:=a_st) (a_st':=a) (o:=o0) (p:=p).
+       concludes.
+       destruct_conjs.
+       specialize IHa2 with (a_st := a) (a_st':=a0) (o:=o1) (p:=p).
+       concludes.
+       subst.
+       ff; eauto. 
+  -
+    df.
+    tauto.
+  -
+    df.
+    tauto. 
+
+        *)
+       
+Defined.
+
+Ltac do_ba_st_const :=
+  let tac := (eapply ba_const; eauto) in
+  repeat (
+      match goal with
+      | [H: build_app_comp _ _ ?a_st = (_, ?a0) |- _] =>
+        assert_new_proof_by (a_st = a0) tac
+      (*
+             destruct gen_const with (e:=ee) (et:=?et) (a:=?A) (a':=?B) (o:=?o);
+             try eassumption *)
+      end);
+  subst.
+
+(*
+Lemma mt_not_mt : forall e t p,
+    e <> mt ->
+    eval t p e <> mt.
+Proof.
+Admitted.
+
+Lemma evMappedExtra : forall a p e a_st,
+    evMapped (eval (unanno a) p e) a_st ->
+    evMapped (eval (unanno a) p mt) a_st.
+Proof.
+Admitted.
+*)
+
+Lemma allMappedSub' : forall a a_st e p,
+    allMapped a a_st p e ->
+    allMapped a a_st p mt.
+Proof.
+  induction a; intros.
+  -
+    destruct a.
+    +
+      allMappedFacts.
+      econstructor.
+      econstructor.
+    +
+      allMappedFacts.
+      econstructor.
+      econstructor.
+      reflexivity.
+      eexists.
+      eauto.
+    +
+      allMappedFacts.
+      econstructor.
+      econstructor.
+      reflexivity.
+      eexists.
+      eauto.
+  -
+    allMappedFacts.
+    df.
+    econstructor.
+    reflexivity.
+    reflexivity.
+    eauto.
+  -
+    allMappedFacts.
+    assert (allMapped a1 a_st p mt) by eauto.
+    econstructor.
+    eassumption.
+    eassumption.
+Defined.
+
+
+Lemma allMappedSub : forall a a_st t p n,
+    allMapped a a_st p (eval t n mt) ->
+    allMapped a a_st p mt.
+Proof.
+  intros.
+  eapply allMappedSub'; eauto.
+Defined.
+
+Lemma build_app_some : forall a a_st p,
+    allMapped a a_st p mt ->
+    exists o, build_app_comp a p a_st = (Some o, a_st).
+Proof.
+  intros.
+  generalizeEverythingElse a.
+  induction a; intros.
+  -
+    destruct a;
+      try (cbn; df; eauto; tauto).
+    +
+      cbn.
+      df.
+      allMappedFacts.
+      debound.
+      subst'.
+      df.
+      eauto.
+    +
+      cbn.
+      df.
+      allMappedFacts.
+      debound.
+      subst'.
+      df.
+      eauto.
+  -
+    cbn.
+    df.
+    allMappedFacts.
+    edestruct IHa.
+    eassumption.
+    destruct_conjs.
+    simpl in *.
+    df.
+    subst'.
+    df.
+    eauto.
+  -
+    allMappedFacts.
+    specialize IHa1 with (a_st:=a_st) (p:=p).
+    specialize IHa2 with (a_st:=a_st) (p:=p).
+    assert (allMapped a2 a_st p mt).
+    eapply allMappedSub'; eauto.
+    repeat concludes.
+    destruct_conjs.
+    df.
+
+    destruct a2;
+      try (subst'';
+           df;
+           eauto).
+    
+    +
+      destruct a;
+        try (subst'; df; eauto).
+
+        (*
+      ++
+        subst'.
+        df.
+        (*
+        cbn in *.
+        unfold bind in H0.
+        cbn in H0.
+        break_let.
+        break_let.
+        break_let.
+        break_let.
+        invc H0. *)
+        allMappedFacts.
+        debound.
+        haaa. *)
+      ++
+        df.
+        allMappedFacts.
+        debound.
+        subst'.
+        df.
+        do_ba_st_const.
+        (*
+        assert (a4 = a).
+        {
+          eapply ba_const; eauto.
+        } *)
+        subst.
+        subst'.
+        df.
+        eauto.
+      
+        
+      
+
+(*
+  -
+    df.
+    eauto.
+  -
+    df.
+    eauto. *)
+Defined.
+
+Lemma ev_shape_transitive : forall e e' et et',
+    Ev_Shape e et ->
+    Ev_Shape e' et ->
+    Ev_Shape e et' ->
+    Ev_Shape e' et'.
+Proof.
+  intros.
+  generalizeEverythingElse e.
+  induction e; destruct et; intros;
+    try repeat evShapeFacts; eauto; tauto.
+Defined.
+
+Lemma evShape_sub : forall a e1 e2 n1 et a_st v0 x vm_st vm_st',
+    Ev_Shape e2 (eval (unanno a) n1 et) ->
+    build_app_comp a n1 a_st = (Some v0, a_st) ->
+    v0 vm_st = (Some x, vm_st') ->
+    e2 = st_ev vm_st ->
+    e1 = st_ev vm_st' ->
+    Ev_Shape e1 et.
+Proof.
+  intros.
+  generalizeEverythingElse a.
+  induction a; intros.
+  -
+    destruct a.
+    +
+      ff; eauto.
+    +
+      df.
+      dosome.
+      ff.
+      vmsts.
+      df.
+      evShapeFacts.
+      df.
+      eassumption.
+    +
+      df.
+      dosome.
+      ff.
+      vmsts.
+      df.
+      evShapeFacts.
+      df.
+      eassumption.
+  -
+    df.
+    eauto.
+  -
+    df.
+    destruct a2 eqn:asp_eq.
+    +
+      destruct a eqn:a2_eq.
+      ++
+        doit.
+
+        destruct v0.
+        destruct vm_st.
+        destruct vm_st'.
+        
+        
+        simpl.
+        simpl in H.  
+        (*simpl in *. *)
+        
+        do_ba_st_const.
+        eapply IHa1;
+          [ eapply IHa2;
+            try (simpl; eassumption);
+            try tauto | eassumption | eassumption | tauto | tauto].
+
+      ++
+        doit.
+        amsts.
+
+        simpl.
+        simpl in H.
+        do_ba_st_const.
+
+        eapply IHa1;
+          [ eapply IHa2;
+            try (simpl; eassumption);
+            try tauto | eassumption | eassumption | tauto | tauto].
+
+      ++
+
+        doit.
+
+        domap.
+        do_pair.
+            
+        assert (exists o, build_app_comp (aasp r0 SIG) n1 a0 = (Some o, a0)).
+        { eapply build_app_some.
+          econstructor.
+          econstructor.
+          reflexivity.
+          eexists.
+          econstructor.
+          eauto.
+        }
+        destruct_conjs.
+        
+        do_ba_st_const.
+
+        doit.
+            
+        subst.
+        cbn in H.
+
+        assert (exists x y, H1 vm_st = (Some x, y)).
+        {
+          cbn in H2.
+          df.
+          dosome.
+          eauto.
+        }
+        destruct_conjs.
+        
+        eapply IHa1.
+        eapply IHa2.
+        eassumption.
+        eassumption.
+        eassumption.
+        reflexivity.
+        reflexivity.
+        eassumption.
+        eassumption.
+        simpl.
+        destruct vm_st.
+        simpl in Heqp5.
+        destruct H5.
+        simpl.
+        cbn in H2.
+        repeat break_let.
+        unfold bind in H2.
+        simpl in H2.
+        cbn in H2.
+        repeat break_let.
+              
+        invc Heqp0.
+        subst''.
+        
+        unfold ret in *.
+        Print do_pair.
+        do_pair.
+        do_pair.
+        doit.
+        reflexivity.
+        reflexivity.
+
+    +
+      doit.
+
+      amsts.
+      simpl.
+      simpl in H.
+      do_ba_st_const.
+      eapply IHa1.
+      eapply IHa2.
+      simpl.
+      eassumption.
+      eassumption.
+      eassumption.
+      tauto.
+      tauto.
+      eassumption.
+      eassumption.
+      tauto.
+      tauto.
+
+    +
+
+      doit.
+
+      amsts.
+      simpl.
+      simpl in H.
+      do_ba_st_const.
+      eapply IHa1.
+      eapply IHa2.
+      simpl.
+      eassumption.
+      eassumption.
+      eassumption.
+      tauto.
+      tauto.
+      eassumption.
+      eassumption.
+      tauto.
+      tauto.
+
+      Unshelve.
+      eauto.
+Defined.
+
+Lemma build_app_run_some : forall a p a_st x v_st et e,
+    e = st_ev v_st ->
+    Ev_Shape e (eval (unanno a) p et) ->
+    (*allMapped a a_st p et -> *)
+    build_app_comp a p a_st = (Some x, a_st) ->
+    exists y v, (x v_st = (Some y, v)).
+Proof.
+  intros.
+  generalizeEverythingElse a.
+  induction a; intros.
+  -
+    destruct a;
+      try evShapeFacts.
+    +
+      df.
+      eauto.    
+    +
+      df.
+      doit.
+      (*
+      dosome.
+      df. *)
+      ff.
+
+      ++
+        eauto.
+      ++
+        vmsts.
+        df.
+        evShapeFacts.
+        solve_by_inversion.
+    +
+      df.
+      doit.
+
+      ff.
+      ++
+        eauto.
+      ++
+        vmsts.
+        df.
+        evShapeFacts.
+        solve_by_inversion.
+        (*
+    +
+      df.
+      dosome.
+      df.
+
+      repeat break_match; try solve_by_inversion.
+      ++
+        df.
+        eauto.
+      ++
+        df.
+        vmsts.
+        df.
+        evShapeFacts.
+        df. *)
+  -
+    df.
+    eauto.
+  -
+    vmsts.
+    df.
+    subst.
+    df.
+
+    destruct a2 eqn:a2_eq.
+    +
+      destruct a eqn:a_eq.
+      ++
+        
+
+
+        
+(*
+        doit. *)
+
+
+        (*doit. *)
+        
+        
+        dosome_eqj.
+        dosome_eqj.
+        repeat break_let.
+
+        do_pair.
+
+        dosome_eqj.
+        do_pair.
+        
+        
+        do_ba_st_const.
+
+        edestruct IHa2 with
+            (v_st:=
+               {|
+                st_ev := st_ev;
+                st_trace := st_trace;
+                st_pl := st_pl;
+                st_store := st_store |}) . 
+        reflexivity.
+        eassumption.
+        eassumption.
+        destruct_conjs.
+        subst''.
+        repeat break_let.
+        
+        amsts.
+
+        edestruct IHa1 (*with
+            (v_st:=
+                {|
+                st_ev := st_ev2;
+                st_trace := st_trace2;
+                st_pl := st_pl2;
+                st_store := st_store2 |})*).
+        reflexivity.
+        eapply evShape_sub.
+        eassumption.
+        eassumption.
+        eassumption.
+        tauto.
+        tauto.
+        eassumption.
+        destruct_conjs.
+        subst''.
+        repeat do_pair.
+        eauto.
+
+      ++
+
+        dosome_eq hi.
+        dosome_eq hey.
+        repeat break_let.
+
+        do_pair.
+
+        dosome_eq hey.
+        do_pair.
+        do_ba_st_const.
+
+        edestruct IHa2 with
+            (v_st:=
+               {|
+                st_ev := st_ev;
+                st_trace := st_trace;
+                st_pl := st_pl;
+                st_store := st_store |}) . 
+        reflexivity.
+        eassumption.
+        eassumption.
+        destruct_conjs.
+        subst''.
+        repeat break_let.
+        Print vmsts.
+
+
+        amsts.
+
+        edestruct IHa1 (*with
+            (v_st:=
+                {|
+                st_ev := st_ev2;
+                st_trace := st_trace2;
+                st_pl := st_pl2;
+                st_store := st_store2 |})*).
+        reflexivity.
+        eapply evShape_sub.
+        eassumption.
+        eassumption.
+        eassumption.
+        tauto.
+        tauto.
+        eassumption.
+        destruct_conjs.
+        subst''.
+        do_pair.
+        inversion Heqp0.
+        eauto.
+      ++
+        do_ba_st_const.
+        df.
+        dosome_eq hi.
+        df.
+        dosome_eq hey.
+        df.
+        
+        simpl in H0.
+        evShapeFacts.
+        df.
+        do_ba_st_const.
+        vmsts.
+        edestruct IHa1 with
+            (v_st:=
+               {|
+            st_ev := e;
+            st_trace := st_trace ++ [umeas n 0 n3 [encodeEv e; bs]];
+            st_pl := st_pl;
+            st_store := st_store |}).
+        reflexivity.
+        eassumption.
+        eassumption.
+        destruct_conjs.
+        vmsts.
+        destruct o3.
+        +++
+          inversion Heqp5.
+          eauto.
+        +++
+          df.
+          Lemma contratra : forall x (f:EvidenceC -> EvidenceC) (vmst vmst':vm_st),
+            x = (None, vmst) ->
+            x = (Some f, vmst') ->
+            False.
+          Proof.
+            intros.
+            rewrite H in *.
+            solve_by_inversion.
+          Defined.
+
+          exfalso.
+          eapply contratra; eauto.
+
+    +
+
+              dosome_eq hi.
+        dosome_eq hey.
+        repeat break_let.
+
+        do_pair.
+
+        dosome_eq hey.
+        do_pair.
+        do_ba_st_const.
+
+        edestruct IHa2 with
+            (v_st:=
+               {|
+                st_ev := st_ev;
+                st_trace := st_trace;
+                st_pl := st_pl;
+                st_store := st_store |}) . 
+        reflexivity.
+        eassumption.
+        eassumption.
+        destruct_conjs.
+        subst''.
+        repeat break_let.
+        Print vmsts.
+
+
+        amsts.
+
+        edestruct IHa1 (*with
+            (v_st:=
+                {|
+                st_ev := st_ev2;
+                st_trace := st_trace2;
+                st_pl := st_pl2;
+                st_store := st_store2 |})*).
+        reflexivity.
+        eapply evShape_sub.
+        eassumption.
+        eassumption.
+        eassumption.
+        tauto.
+        tauto.
+        eassumption.
+        destruct_conjs.
+        subst''.
+        do_pair.
+        inversion Heqp0.
+        eauto.
+    +
+      dosome_eq hi.
+        dosome_eq hey.
+        repeat break_let.
+
+        do_pair.
+
+        dosome_eq hey.
+        do_pair.
+        do_ba_st_const.
+
+        edestruct IHa2 with
+            (v_st:=
+               {|
+                st_ev := st_ev;
+                st_trace := st_trace;
+                st_pl := st_pl;
+                st_store := st_store |}) . 
+        reflexivity.
+        eassumption.
+        eassumption.
+        destruct_conjs.
+        subst''.
+        repeat break_let.
+        Print vmsts.
+
+
+        amsts.
+
+        edestruct IHa1 (*with
+            (v_st:=
+                {|
+                st_ev := st_ev2;
+                st_trace := st_trace2;
+                st_pl := st_pl2;
+                st_store := st_store2 |})*).
+        reflexivity.
+        eapply evShape_sub.
+        eassumption.
+        eassumption.
+        eassumption.
+        tauto.
+        tauto.
+        eassumption.
+        destruct_conjs.
+        subst''.
+        do_pair.
+        inversion Heqp0.
+        eauto.
+Defined.
+
+
+(*
+Lemma fafafaf : forall e tr p o tr' (x:VM (EvidenceC -> EvidenceC)) a a_st p' p'' o'',
+    build_app_comp a p' a_st = (Some x, a_st) -> 
+    fst (x {| st_ev := e; st_trace := tr; st_pl := p; st_store := o |}) =
+    fst (x {| st_ev := e; st_trace := tr'; st_pl := p''; st_store := o'' |}).
+Proof.
+Admitted.
+*)
+Print AnnoTerm.
+
+(*
+Lemma same_ev_shape : forall a a_st e e_res vm_st p et e' t q,
+    allMapped a a_st p et ->
+    (*p = am_pl a_st -> *)
+    (*Ev_Shape e' (eval (unanno t) q mt) -> *)
+
+    Ev_Shape e'' (eval (unano t) q mt) ->
+    e'' = (run_app_comp t q a_st e') mtc
+
+    vm_st = run_vm a {| st_ev := e'; st_trace := []; st_pl := 0; st_store := [] |} ->
+    e_res = st_ev vm_st ->
+    Ev_Shape e_res e_res_t ->
+    (*e_res_t = eval (unanno a) 0 et ->*)
+    (*Ev_Shape e'' et ->*)
+    e = (run_app_comp a p a_st e_res) e''  (*TODO: remove func, just add extra lseq term for initial appraising initial evidence *) ->
+    Ev_Shape e e_res_t.
+ *)
+
+
+(*
+Lemma dood : forall t vm_st vm_st' e e'' e' p a_st x0 x1 new_vmst new_vmst',
+    build_comp t vm_st = (Some tt, vm_st') ->
+    e = st_ev vm_st ->
+    e' = st_ev vm_st' ->
+    build_app_comp t p a_st = (Some x0, a_st) ->
+    x0 new_vmst = (Some x1, new_vmst') ->
+    e' = st_ev new_vmst -> 
+    e'' = st_ev new_vmst' ->
+    e = e''.
+Proof.
+Admitted.
+*)
+
+(*
+Lemma evShapeAt : forall e et a n,
+    well_formed a -> 
+    Ev_Shape e et ->
+    Ev_Shape (toRemote (unanno a) e) (eval (unanno a) n et).
+Proof.
+  intros.
+  eapply multi_ev_eval.
+  eassumption.
+  apply build_comp_at.
+  eassumption.
+  reflexivity.
+  Unshelve.
+  exact [].
+Defined.
+*)
+
+Lemma same_ev_shape: forall t vmst vmst' e e_res et e_res_t p a_st x new_vmst new_vmst' f e'' app_ev,
+  well_formed t ->
+  build_comp t vmst = (Some tt, vmst') ->
+  e = st_ev vmst ->
+  Ev_Shape e et ->
+  e_res = st_ev vmst' ->
+  Ev_Shape e_res e_res_t ->
+  build_app_comp t p a_st = (Some x, a_st) -> (* x : VM (EvidenceC -> EvidenceC) *)
+  runSt new_vmst x = (Some f, new_vmst') ->
+  Ev_Shape e'' et ->
+  app_ev = f e'' ->
+  Ev_Shape app_ev e_res_t.
+Proof.
+  intros.
+  subst.
+  vmsts.
+  simpl in *.
+  df.
+  generalizeEverythingElse t.
+  induction t; intros;
+    try do_wf_pieces.
+  -
+    destruct r.
+    destruct a.
+    +
+      df.
+      dosome.
+     (* evShapeFacts. 
+      haaa.
+      econstructor. *)
+      eapply ev_shape_transitive.
+      apply H2.
+      eassumption.
+      eassumption.
+
+    +
+      df.
+      dosome.
+      evShapeFacts.
+      haaa.
+      econstructor.
+      eapply ev_shape_transitive.
+      apply H2.
+      eassumption.
+      eassumption.
+    +
+       df.
+      dosome.
+      evShapeFacts.
+      haaa.
+      econstructor.
+      eapply ev_shape_transitive.
+      apply H2.
+      eassumption.
+      eassumption.
+      (* HSH case
+    +
+      df.
+      dosome.
+      evShapeFacts.
+     (* haaa. *)
+      econstructor.
+      eapply ev_shape_transitive.
+      apply H1.
+      eassumption.
+      eassumption. *)
+  -
+
+    df.
+    dohtac.
+    df.
+    eapply IHt.
+    eassumption.
+    apply build_comp_at.
+    apply H2.
+    eassumption.
+    eassumption.
+    eassumption.
+    eassumption.
+  -
+    df.
+    dosome.
+    destruct t2 eqn:t2_eq.
+    ++
+      vmsts.
+      destruct a eqn:a_eq.
+      +++
+        break_match.
+        dosome.
+        do_ba_st_const.
+        (*break_match; try solve_by_inversion. *)
+        df.
+        (*evShapeFacts.
+        econstructor. *)
+        eapply IHt1.
+        eassumption.
+        eassumption.
+        eassumption.
+        eassumption.
+        eassumption.
+        eassumption.
+        eassumption.
+
+      +++
+        break_match.
+        dosome.
+        do_ba_st_const.
+        break_match; try solve_by_inversion.
+        df.
+        evShapeFacts.
+        econstructor.
+        eapply IHt1.
+        eassumption.
+        eassumption.
+        eassumption.
+        eassumption.
+        eassumption.
+        eassumption.
+        eassumption.
+      +++
+        break_match.
+        dosome.
+        do_ba_st_const.
+        break_match; try solve_by_inversion.
+        df.
+        evShapeFacts.
+        econstructor.
+        eapply IHt1.
+        eassumption.
+        eassumption.
+        eassumption.
+        eassumption.
+        eassumption.
+        eassumption.
+        eassumption.
+    ++
+
+      dosome_eq hi.
+      dosome_eq hey.
+      repeat break_let.
+
+      do_pair.
+
+      dosome_eq hey.
+      do_pair.
+      do_ba_st_const.
+      break_match; try solve_by_inversion.
+      dosome_eq heey.
+      repeat break_let.
+      subst.
+      do_pair.
+      dosome_eq hii.
+      do_pair.
+      amsts.
+      do_pl_immut.
+
+      eapply IHt2.
+      eassumption.
+      eassumption.
+      eapply multi_ev_eval.
+      apply H1.
+      eassumption.
+      eassumption.
+      reflexivity.
+      eassumption.
+      eassumption.
+      eassumption.
+
+      eapply IHt1.
+      eassumption.
+      eassumption.
+      eassumption.
+      eapply multi_ev_eval.
+      apply H1.
+      eassumption.
+      eassumption.
+      reflexivity.
+      eassumption.
+      eassumption.
+      eassumption.
+    ++
+      dosome_eq hi.
+      dosome_eq hey.
+      repeat break_let.
+
+      do_pair.
+
+      dosome_eq hey.
+      do_pair.
+      do_ba_st_const.
+      break_match; try solve_by_inversion.
+      dosome_eq heey.
+      repeat break_let.
+      subst.
+      do_pair.
+      dosome_eq hii.
+      do_pair.
+      amsts.
+      do_pl_immut.
+
+      eapply IHt2.
+      eassumption.
+      eassumption.
+      eapply multi_ev_eval.
+      apply H1.
+      eassumption.
+      eassumption.
+      reflexivity.
+      eassumption.
+      eassumption.
+      eassumption.
+
+      eapply IHt1.
+      eassumption.
+      eassumption.
+      eassumption.
+      eapply multi_ev_eval.
+      apply H1.
+      eassumption.
+      eassumption.
+      reflexivity.
+      eassumption.
+      eassumption.
+      eassumption.
+      Unshelve.
+      eauto.
+      eauto.
+      exact (aasp (0,0) (ASPC 1 [])).
+      exact mtc.
+      eauto.
+      eauto.
+      exact (aasp (0,0) (ASPC 1 [])).
+      exact mtc.
+      eauto.
+      eauto.
+Defined.
+      
+(* OLD EV_SHAPE LEMMA 
+Lemma same_ev_shape : forall a a_st p et vm_st vm_st' e_res e_res_t e' e'' e,
+    allMapped a a_st p et ->
+    well_formed a ->
+    vm_st' = run_vm a vm_st ->
+    p = st_pl vm_st ->
+    e_res = st_ev vm_st' ->
+    Ev_Shape e_res e_res_t ->
+    e' = st_ev vm_st ->
+    Ev_Shape e' et ->
+    Ev_Shape e'' et ->
+    (*e_res_t = eval (unanno a) 0 et ->*)
+    e = (run_app_comp a p a_st e_res) e''
+    (*TODO: remove func, just add extra lseq term for initial appraising initial evidence *) ->
+    Ev_Shape e e_res_t.
+ *)
+
+Inductive evidenceEvent: Ev -> Prop :=
+| uev: forall n p i args, evidenceEvent (umeas n p i args)
+(*| sev: forall n p, evidenceEvent (sign n p)
+| hev: forall n p, evidenceEvent (hash n p)*) .
+
+
+Definition measEvent (t:AnnoTerm) (p:Plc) (ev:Ev) : Prop :=
+  events t p ev /\ evidenceEvent ev.
+
+Inductive appEvent : Ev -> AM_St -> Ev -> Prop :=
+| aeu : forall p q i i' n n' m args st,
+    m = st_aspmap st ->
+    bound_to m (p,i) i' ->
+    appEvent (umeas n p i args) st (umeas n' q i' ([n] ++ args)).
+
+Ltac measEventFacts :=
+  match goal with
+  | [H: measEvent _ _ _ |- _] => invc H
+  end.
+
+Ltac evEventFacts :=
+  match goal with
+  | [H: evidenceEvent _ |- _] => invc H
+  end.
+
+Ltac invEvents :=
+  match goal with
+  | [H: events _ _ _  |- _] => invc H
+  end.
+    
+
+Lemma measEventAt' : forall t n p q ev,
+    measEvent (snd (anno (att n t) q)) p ev ->
+    measEvent (snd (anno t (S q))) n ev.
+Proof.
+
+  induction t; intros;
+    try (
+      df;
+      measEventFacts;
+      evEventFacts;
+      invEvents;
+      invEvents;
+      try (repeat econstructor; eauto; tauto)).
+Defined.
+
+Ltac dosome_eq' y :=
+  match goal with
+  | H:match ?x with
+      | _ => _
+      end _ = (Some _, _) |- _ => destruct x eqn:y; try solve_by_inversion
+  end.
+
+Lemma trace_cumul : forall  t e a_st a_st' v tr tr' p n n' o o' e' o0,
+    build_app_comp t p a_st = (Some v, a_st') ->
+    v    {| st_ev := e;  st_trace := tr;  st_pl := n;  st_store := o |} =
+    (Some o0, {| st_ev := e'; st_trace := tr'; st_pl := n'; st_store := o'|}) ->
+    exists tr'', tr' = tr ++ tr''.
+Proof.
+  induction t; intros.
+  -
+    destruct a.
+    +
+      df.
+      exists [].
+      rewrite app_nil_r.
+      eauto.
+    +
+      
+      df.
+      doit.
+      (*
+      dosome.
+      dosome_eq' hey.
+      df. *)
+      unfold extractUev in *.
+
+      
+      
+      dosome_eq' hi.
+      df.
+      eexists.
+      reflexivity.
+    +
+      df.
+      doit.
+      (*
+      dosome.
+      dosome_eq' hey.
+      df. *)
+      unfold extractSig in *.
+      dosome_eq' hi.
+      df.
+      eexists.
+      reflexivity.
+  -
+    df.
+    do_ba_st_const.
+    eauto.
+  -
+    df.
+    do_ba_st_const.
+    destruct t2.
+    +
+      destruct a.
+      ++
+        doit.
+        amsts.
+        edestruct IHt1.
+        eassumption.
+        eassumption.
+        subst.
+        edestruct IHt2.
+        eassumption.
+        eassumption.
+        subst.
+        rewrite <- app_assoc.
+        eexists.
+        eauto.
+      ++
+        doit.
+        amsts.
+        edestruct IHt1.
+        eassumption.
+        eassumption.
+        subst.
+        edestruct IHt2.
+        eassumption.
+        eassumption.
+        subst.
+        rewrite <- app_assoc.
+        eexists.
+        eauto.
+      ++
+
+        doit.
+
+        
+        simpl in Heqp6.
+        dosome_eq' hihihihi.
+        do_pair.
+        (*
+        simpl in heyyyy. *)
+        unfold extractSig in *.
+        dosome_eq' ho.
+        unfold ret in *.
+        do_pair.
+
+        edestruct IHt1.
+        eassumption.
+        eassumption.
+        subst.
+        eexists.
+        rewrite app_assoc.
+        reflexivity.
+    +
+      doit.
+      amsts.
+      edestruct IHt1.
+      eassumption.
+      eassumption.
+      subst.
+      edestruct IHt2.
+      eassumption.
+      eassumption.
+      subst.
+      rewrite <- app_assoc.
+      eexists.
+      eauto.
+    +
+      doit.
+      amsts.
+      edestruct IHt1.
+      eassumption.
+      eassumption.
+      subst.
+      edestruct IHt2.
+      eassumption.
+      eassumption.
+      subst.
+      rewrite <- app_assoc.
+      eexists.
+      eauto.
+Defined.
+
+Ltac do_cumul2 :=
+    match goal with
+    | [
+      H: ?v {| st_ev := _; st_trace := ?tr1; st_pl := _; st_store := _ |} =
+         (_, {| st_ev := _; st_trace := ?tr1'; st_pl := _; st_store := _ |}),
+     H2: build_app_comp _ _ _ = (Some ?v, _),
+
+     H': ?v2 {| st_ev := _; st_trace := ?tr2; st_pl := _; st_store := _ |} =
+         (_, {| st_ev := _; st_trace := ?tr2'; st_pl := _; st_store := _ |}),
+    H'2: build_app_comp _ _ _ = (Some ?v2, _) |- _] =>
+
+      assert (exists tr'' : list Ev, tr1' = tr1 ++ tr'')by (eapply trace_cumul; [apply H2 | apply H]) ;
+      assert (exists tr'' : list Ev, tr2' = tr2 ++ tr'')by (eapply trace_cumul; [apply H'2 | apply H'])
+    end.
+
+
+Ltac do_cumul4 :=
+    match goal with
+    | [
+      H: ?v {| st_ev := _; st_trace := ?tr1; st_pl := _; st_store := _ |} =
+         (_, {| st_ev := _; st_trace := ?tr1'; st_pl := _; st_store := _ |}),
+     H2: build_app_comp _ _ _ = (Some ?v, _),
+             
+     H'': ?v {| st_ev := _; st_trace := ?tr3; st_pl := _; st_store := _ |} =
+         (_, {| st_ev := _; st_trace := ?tr3'; st_pl := _; st_store := _ |}),
+     H''': ?v2 {| st_ev := _; st_trace := ?tr31; st_pl := _; st_store := _ |} =
+         (_, {| st_ev := _; st_trace := ?tr31'; st_pl := _; st_store := _ |}),
+
+     H': ?v2 {| st_ev := _; st_trace := ?tr2; st_pl := _; st_store := _ |} =
+         (_, {| st_ev := _; st_trace := ?tr2'; st_pl := _; st_store := _ |}),
+    H'2: build_app_comp _ _ _ = (Some ?v2, _) |- _] =>
+
+      assert (exists tr'' : list Ev, tr1' = tr1 ++ tr'')by (eapply trace_cumul; [apply H2 | apply H]) ;
+      assert (exists tr'' : list Ev, tr2' = tr2 ++ tr'')by (eapply trace_cumul; [apply H'2 | apply H']);
+      assert (exists tr'' : list Ev, tr3' = tr3 ++ tr'')by (eapply trace_cumul; [apply H2 | apply H'']) ;
+      assert (exists tr'' : list Ev, tr31' = tr31 ++ tr'')by (eapply trace_cumul; [apply H'2 | apply H'''])
+    end.
+
+Ltac do_cumul2' :=
+    match goal with
+    | [
+      H: ?v {| st_ev := _; st_trace := ?tr1; st_pl := _; st_store := _ |} =
+         (_, {| st_ev := _; st_trace := ?tr1'; st_pl := _; st_store := _ |}),
+     H2: build_app_comp _ _ _ = (Some ?v, _),
+     H': ?v {| st_ev := _; st_trace := ?tr2; st_pl := _; st_store := _ |} =
+           (_, {| st_ev := _; st_trace := ?tr2'; st_pl := _; st_store := _ |}) |- _] =>
+
+      assert (exists tr'' : list Ev, tr1' = tr1 ++ tr'')by (eapply trace_cumul; [apply H2 | apply H]) ;
+      assert (exists tr'' : list Ev, tr2' = tr2 ++ tr'')by (eapply trace_cumul; [apply H2 | apply H'])
+    end.
+
+Ltac do_cumul1 :=
+    match goal with
+    | [
+      H: ?v {| st_ev := _; st_trace := ?tr1; st_pl := _; st_store := _ |} =
+         (_, {| st_ev := _; st_trace := ?tr1'; st_pl := _; st_store := _ |}),
+     H2: build_app_comp _ _ _ = (Some ?v, _) |- _] =>
+
+      assert (exists tr'' : list Ev, tr1' = tr1 ++ tr'')by (eapply trace_cumul; [apply H2 | apply H])
+    end.
+
+Ltac do_cumul := first [do_cumul4 | do_cumul2 | do_cumul2' | do_cumul1]; destruct_conjs.
+
+Lemma isnil{A:Type} : forall (ls xs : list A),
+    ls = ls ++ xs ->
+    xs = [].
+Proof.
+  intros.
+  assert (ls = ls ++ []).
+  {
+    rewrite app_nil_r.
+    tauto.
+  }
+  rewrite H0 in H at 1.
+  eapply app_inv_head; eauto.
+Defined.
+
+Ltac dothat :=
+  unfold StVM.st_ev, StVM.st_pl, StVM.st_trace, StVM.st_store in *;
+  try unfold st_ev in *;
+  try unfold st_pl in *;
+  try unfold st_trace in *;
+  try unfold st_store in *.
+
+Ltac ff' :=
+  repeat break_match; try solve_by_inversion.
+
+Ltac doex := 
+  unfold extractUev, extractSig in *;
+  ff';
+  unfold ret in *; doit.
+
+Ltac do_inv_head :=
+  let tac := (eapply app_inv_head; eauto) in
+  repeat
+    match goal with
+    | [H: ?ls ++ ?xs = ?ls ++ ?ys |- _] => assert_new_proof_by (xs = ys) tac
+    end.
+
+
+(*
+Lemma gogo' : forall t p a a' o_res o_res' v1 e1' p1 p1' o1 o1' e2 e2' tr2 p2 p2' o2 o2' tr1 x0 x1,
+    build_app_comp t p a = (Some v1, a') ->
+    v1 {| st_ev := e2; st_trace := tr1; st_pl := p1; st_store := o1 |} =
+    (Some o_res, {| st_ev := e1'; st_trace := tr1 ++ x1; st_pl := p1'; st_store := o1' |}) ->
+    v1 {| st_ev := e2; st_trace := tr2; st_pl := p2; st_store := o2 |} =
+    (Some o_res', {| st_ev := e2'; st_trace := tr2 ++ x0; st_pl := p2'; st_store := o2' |}) ->
+    x0 = x1.
+Proof.
+  induction t; intros.
+  -
+    destruct r; destruct a.
+    +
+      df. 
+      assert (x1 = []) by (eapply isnil; eauto).
+      assert (x0 = []) by (eapply isnil; eauto).
+      congruence.
+    +
+      df.
+      doit.
+      domap.
+      doit.
+      dothat.
+      doex.
+      do_inv_head.
+      congruence.
+    +
+      df.
+      doit.
+      domap.
+      doit.
+      dothat.
+      doex.
+      do_inv_head.
+      congruence.
+  -
+    df.
+    eauto.
+  -
+    df.
+    destruct r.
+    subst.
+    destruct t2.
+    +
+      doit.
+      destruct a0.
+      ++
+        doit.
+
+        cbn in Heqp0.
+        repeat break_let.
+        doex.
+        eauto.
+      ++
+        doit.
+        cbn in Heqp0.
+        df.
+        doit.
+        domap.
+        doit.
+        doex.
+        
+        repeat break_let.
+        doex.
+        doit.
+        df.
+        doit.
+        subst.
+        invc Heqe.
+        eauto.
+        do_cumul.
+        assert (x0 = [umeas n4 0 n1 (b :: l)] ++ H0).
+        {
+          admit.
+        }
+
+        assert (x1 = [umeas n4 0 n1 (b :: l)] ++ H1).
+        {
+          admit.
+        }
+        assert (H0 = H1).
+        {
+          admit.
+        }
+        subst.
+        congruence.
+      ++
+        doit.
+        doex.
+        dothat.
+        subst.
+        invc Heqe4.
+
+        do_cumul.
+        assert (x0 = [umeas n 0 n3 [encodeEv e; b]] ++ H).
+        {
+          admit.
+        }
+
+        assert (x1 = [umeas n 0 n3 [encodeEv e; b]] ++ H0).
+        {
+          admit.
+        }
+        assert (H = H0).
+        {
+          admit.
+        }
+        subst.
+        congruence.
+    +
+      doit.
+      cbn in Heqp0.
+      amsts.
+      do_cumul.
+      subst.
+      assert (x0 = H3 ++ H).
+      {
+        admit.
+      }
+      subst.
+      assert (x1 = H0 ++ H4).
+      {
+        admit.
+      }
+      subst.
+      assert (H = H4).
+      eapply IHt1.
+      eassumption.
+      rewrite app_assoc in *.
+      eassumption.
+      repeat rewrite app_assoc in *.
+      assert (st_ev = st_ev0).
+      {
+        admit.
+      }
+      subst.
+      eassumption.
+      subst.
+      assert (H3 = H0) by eauto.
+      subst.
+      reflexivity.
+   +
+      doit.
+      
+      (*cbn in Heqp0. *)
+      amsts.
+      do_cumul.
+      subst.
+      assert (x0 = H3 ++ H).
+      {
+        admit.
+      }
+      subst.
+      assert (x1 = H0 ++ H4).
+      {
+        admit.
+      }
+      subst.
+      assert (H = H4).
+      eapply IHt1.
+      eassumption.
+      rewrite app_assoc in *.
+      eassumption.
+      repeat rewrite app_assoc in *.
+      assert (st_ev = st_ev0).
+      {
+        admit.
+      }
+      subst.
+      eassumption.
+      subst.
+      assert (H3 = H0) by eauto.
+      subst.
+      reflexivity.
+      Unshelve.
+      eauto.
+        
+    
+    
+      
+      
+      
+
+      
+      
+      
+
+      
+      
+
+
+
+
+
+
+
+
+
+
+
+(*
+
+  
+  assert (Ev_Shape e et).
+  eapply gen_ev_shape; eauto.
+  generalizeEverythingElse e.
+
+  induction e;
+    intros;
+    evShapeFacts;
+    try
+      ( df;
+        dosome;
+        haaa;
+        do_cumul;
+        repeat subst'';                                                           
+        repeat dof;
+        assert (H0 = H1) by ( eapply IHe; eauto);
+        congruence);
+    try
+      ( df;
+        dosome;
+        repeat break_match; try solve_by_inversion;
+        df;
+        eauto).
+  -
+    df.
+    assert (x0 = []).
+    eapply lista; eauto.
+    assert (x1 = []).
+    eapply lista; eauto.
+    congruence.
+  -
+    df.
+    dosome.
+    repeat break_match; try solve_by_inversion.
+    vmsts.
+
+    edestruct trace_cumul.
+    apply Heqp.
+    apply Heqp1.
+    subst.
+
+    edestruct trace_cumul.
+    apply Heqp.
+    apply Heqp3.
+    subst.
+
+    assert (x = x2).
+    eauto.
+    subst.
+
+    edestruct trace_cumul.
+    apply Heqp0.
+    apply Heqp4.
+    rewrite H in *.
+
+    edestruct trace_cumul.
+    apply Heqp0.
+    apply Heqp2.
+    rewrite H0 in *.
+
+    assert (x = x3).
+    eauto.
+    subst.
+
+    assert (x0 = x2 ++ x3).
+    {
+      assert ((tr2 ++ x2) ++ x3 = tr2 ++ (x2 ++ x3)).
+      {
+        rewrite app_assoc.
+        reflexivity.
+      }
+      rewrite H1 in H.
+      eapply app_inv_head.
+      eassumption.
+    }
+
+    assert (x1 = x2 ++ x3).
+    {
+      assert ((tr1 ++ x2) ++ x3 = tr1 ++ (x2 ++ x3)).
+      {
+        rewrite app_assoc.
+        reflexivity.
+      }
+      rewrite H2 in H0.
+      eapply app_inv_head.
+      eassumption.
+    }
+    congruence.
+    
+  -
+    df.
+    dosome.
+    repeat break_match; try solve_by_inversion.
+    vmsts.
+
+    edestruct trace_cumul.
+    apply Heqp.
+    apply Heqp1.
+    subst.
+
+    edestruct trace_cumul.
+    apply Heqp.
+    apply Heqp3.
+    subst.
+
+    assert (x = x2).
+    eauto.
+    subst.
+
+    edestruct trace_cumul.
+    apply Heqp0.
+    apply Heqp4.
+    rewrite H in *.
+
+    edestruct trace_cumul.
+    apply Heqp0.
+    apply Heqp2.
+    rewrite H0 in *.
+
+    assert (x = x3).
+    eauto.
+    subst.
+
+    assert (x0 = x2 ++ x3).
+    {
+      assert ((tr2 ++ x2) ++ x3 = tr2 ++ (x2 ++ x3)).
+      {
+        rewrite app_assoc.
+        reflexivity.
+      }
+      rewrite H1 in H.
+      eapply app_inv_head.
+      eassumption.
+    }
+
+    assert (x1 = x2 ++ x3).
+    {
+      assert ((tr1 ++ x2) ++ x3 = tr1 ++ (x2 ++ x3)).
+      {
+        rewrite app_assoc.
+        reflexivity.
+      }
+      rewrite H2 in H0.
+      eapply app_inv_head.
+      eassumption.
+    }
+    congruence.
+Defined.
+   *)
+Admitted.
+
+
+Lemma gogo : forall t p a a' o_res o_res' v1 e1' p1 p1' o1 o1' e2 e2' tr2 p2 p2' o2 o2' tr1 x0,
+    build_app_comp t p a = (Some v1, a') ->
+    v1 {| st_ev := e2; st_trace := []; st_pl := p1; st_store := o1 |} =
+    (Some o_res, {| st_ev := e1'; st_trace := tr1; st_pl := p1'; st_store := o1' |}) ->
+    v1 {| st_ev := e2; st_trace := tr2; st_pl := p2; st_store := o2 |} =
+    (Some o_res', {| st_ev := e2'; st_trace := tr2 ++ x0; st_pl := p2'; st_store := o2' |}) ->
+    x0 = tr1.
+Proof.
+  intros.
+  eapply gogo'.
+  eassumption.
+  assert (tr1 = [] ++ tr1).
+  simpl.
+  reflexivity.
+  subst''.
+  eassumption.
+  eassumption.
+Defined.
+
+Ltac do_gogo :=
+    match goal with
+    | [
+      H: ?v {| st_ev := _; st_trace := []; st_pl := _; st_store := _ |} =
+         (Some _, {| st_ev := _; st_trace := ?tr1'; st_pl := _; st_store := _ |}),
+     H2: build_app_comp _ _ _ = (Some ?v, _),
+     H': ?v {| st_ev := _; st_trace := ?tr2; st_pl := _; st_store := _ |} =
+           (Some _, {| st_ev := _; st_trace := ?tr2 ++ ?tr2'; st_pl := _; st_store := _ |}) |- _] =>
+
+      assert (tr2' = tr1')by (eapply gogo; [apply H2 | apply H | apply H'])
+    end.
+*)
+
+(*
+Lemma foofoo : forall t f p tr_n p_n o_n a0 a' v e' tr' p' o' e'' tr'' p'' o'',
+    build_app_comp t p a0 = (Some v, a') ->
+    v {| st_ev := e'; st_trace := tr'; st_pl := p'; st_store := o' |} =
+    (Some f, {| st_ev := e''; st_trace := tr''; st_pl := p''; st_store := o'' |}) ->
+    (exists g e3 tr3 p3 o3,
+        v {| st_ev := e'; st_trace := tr_n; st_pl := p_n; st_store := o_n |} =
+        (Some g, {| st_ev := e3; st_trace := tr3; st_pl := p3; st_store := o3 |})).
+Proof.
+Admitted.
+*)
+
+Lemma dood : forall t vm_st vm_st' e e'' e' p a_st x0 x1 new_vmst new_vmst',
+    build_comp t vm_st = (Some tt, vm_st') ->
+    e = st_ev vm_st ->
+    e' = st_ev vm_st' ->
+    build_app_comp t p a_st = (Some x0, a_st) ->
+    x0 new_vmst = (Some x1, new_vmst') ->
+    e' = st_ev new_vmst -> 
+    e'' = st_ev new_vmst' ->
+    e = e''.
+Proof.
+  induction t; intros.
+  -
+    destruct a.
+    +
+      subst.
+      amsts.
+      df.
+      reflexivity.
+    +
+      subst.
+      amsts.
+      df.
+      dosome.
+      reflexivity.
+    +
+      subst.
+      amsts.
+      df.
+      dosome.
+      reflexivity.
+  -
+    subst.
+    amsts.
+    df.
+    dohtac.
+    df.
+    eapply IHt.
+    apply build_comp_at.
+    reflexivity.
+    reflexivity.
+    eassumption.
+    eassumption.
+    tauto.
+    tauto.
+  -
+    subst.
+    amsts.
+    df.    
+    dosome. 
+    destruct t2.
+    +
+      destruct a eqn:aeq.
+      ++
+        doit.
+        (*
+        doit. *)
+        
+        (*
+        dosome_eq hi.
+        dosome_eq hey.
+        repeat break_let.
+        do_pair.
+        dosome_eq hey.
+        do_pair.
+        dosome_eq hey.
+        dosome_eq heyy.
+        repeat break_let.
+        do_pair.
+        dosome_eq heey.
+        do_pair. *)
+        cbn in Heqp2.
+        repeat break_let.
+        unfold ret in *.
+        
+        do_pair.
+        do_pair. 
+        amsts.
+        cbn in Heqp1.
+        do_pair. 
+        eauto.
+      ++
+        doit.
+        (*
+        dosome_eq hi.
+        dosome_eq hey.
+        repeat break_let.
+        do_pair.
+        dosome_eq hey.
+        do_pair.
+        dosome_eq hey.
+        dosome_eq heyy.
+        repeat break_let.
+        do_pair.
+        dosome_eq heey.
+        do_pair. *)
+        amsts.
+        cbn in Heqp2.
+        clear IHt2. df.
+        dosome.
+        haaa.
+      ++
+        clear IHt2.
+        df.
+        dosome.
+        haaa.
+    +
+      doit.
+      (*
+      dosome_eq hi.
+      dosome_eq hey.
+      repeat break_let.
+      do_pair.
+      dosome_eq hii.
+      do_pair.
+      dosome_eq heey.
+      dosome_eq hii.
+      repeat break_let.
+      do_pair.
+      dosome_eq hee.
+      do_pair. *)
+
+      amsts.
+      do_ba_st_const.
+      do_pl_immut.
+
+      assert (st_ev3 = st_ev1).
+      eapply IHt2.
+      eassumption.
+      tauto.
+      tauto.
+      eassumption.
+      eassumption.
+      tauto.
+      tauto.
+      subst.
+
+      eapply IHt1.
+      eassumption.
+      tauto.
+      tauto.
+      eassumption.
+      eassumption.
+      tauto.
+      tauto.
+    +
+      doit.
+      (*
+      dosome_eq hi.
+      dosome_eq hey.
+      repeat break_let.
+      do_pair.
+      dosome_eq hii.
+      do_pair.
+      dosome_eq heey.
+      dosome_eq hii.
+      repeat break_let.
+      do_pair.
+      dosome_eq hee.
+      do_pair. *)
+
+      amsts.
+      do_ba_st_const.
+      do_pl_immut.
+
+      assert (st_ev3 = st_ev1).
+      eapply IHt2.
+      eassumption.
+      tauto.
+      tauto.
+      eassumption.
+      eassumption.
+      tauto.
+      tauto.
+      subst.
+
+      eapply IHt1.
+      eassumption.
+      tauto.
+      tauto.
+      eassumption.
+      eassumption.
+      tauto.
+      tauto.
+      Unshelve.
+      eauto.
+      eauto.
+      exact (aasp (0,0) (ASPC 1 [])).
+      exact mtc.
+      eauto.
+      eauto.
+      exact (aasp (0,0) (ASPC 1 [])).
+      exact mtc.
+      eauto.
+      eauto.
+Defined.
+
+
+
+Lemma appraisal_correct : forall t vmst vmst' p e_res new_vmst new_vmst' a_st x f tr_app ev,
+
+    (*well_formed t -> *)
+    build_comp t vmst = (Some tt, vmst') ->
+    (*e = st_ev vmst ->
+  Ev_Shape e et -> *)
+    p = st_pl vmst ->
+    e_res = st_ev vmst' ->
+    e_res = st_ev new_vmst ->
+    build_app_comp t p a_st = (Some x, a_st) -> (* x : VM (EvidenceC -> EvidenceC) *)
+    runSt new_vmst x = (Some f, new_vmst') ->
+    tr_app = st_trace new_vmst' ->
+    measEvent t p ev ->
+    exists ev', In ev' tr_app /\ appEvent ev a_st ev'.
+Proof.
+  induction t; intros.
+  -
+    destruct a.
+    +
+      measEventFacts.
+      evEventFacts.
+      solve_by_inversion.
+    +
+      measEventFacts.
+      evEventFacts.
+      invEvents.
+      destruct r.
+      simpl.
+      
+      
+      amsts.
+      unfold StVM.st_ev in *.
+      unfold StVM.st_pl in *.
+      unfold StVM.st_trace in *.
+      subst.
+      df.
+      doit.
+      (*
+      
+      dosome_eq hey.
+      do_pair.
+      repeat break_let.
+      do_pair.
+      dosome_eq hey.
+      df. *)
+      dosome_eq' heyy.
+      df.
+      exists (umeas b 0 n1 (b :: args)).
+      split.
+      ++
+        Print In.
+        Search In.
+        eapply in_or_app.
+        right.
+        econstructor. reflexivity.
+      ++
+        assert (b::args = [b] ++ args).
+        reflexivity.
+        rewrite H.
+        econstructor.
+        reflexivity.
+        econstructor.
+        eassumption.
+    +
+      measEventFacts.
+      evEventFacts.
+      solve_by_inversion.
+  -
+    amsts.
+    subst.
+    df.
+    dohtac.
+    df.
+
+    measEventFacts.
+    evEventFacts.
+    invEvents.
+   
+
+    (*
+    Check foofoo.     
+    edestruct foofoo.
+    eassumption.
+    eassumption.
+    destruct_conjs. *)
+
+    Locate build_comp_at.
+    Print build_comp_at.
+
+    edestruct IHt with (vmst:={| st_ev := st_ev3; st_trace := []; st_pl := n; st_store := [] |})
+                       (new_vmst:= {| st_ev := toRemote (unanno t) st_ev3; st_trace := st_trace0; st_pl := st_pl0; st_store := st_store0 |})
+                       (*(new_vmst:={| st_ev := toRemote (unanno t) st_ev3; st_trace := []; st_pl := 0; st_store := [] |})*).
+    
+    apply build_comp_at.
+    simpl.
+    reflexivity.
+    simpl.
+    reflexivity.
+    tauto.
+    simpl.
+    eassumption.
+    eassumption.
+    (*
+    apply H5. *)
+    simpl.
+    reflexivity.
+    simpl.
+    econstructor.
+    eassumption.
+    econstructor.
+
+
+    (*
+    assert (st_trace = st_trace0 ++ H0).
+    {
+      Print do_cumul2'.
+      do_cumul.
+      
+      subst.
+      assert (H8 = H9).
+      {
+        eapply gogo; eauto.
+      }
+      subst.
+      simpl.
+      reflexivity.
+    } *)
+
+    (*
+    do_cumul. *)
+
+    (* 
+    simpl in H11.
+    subst.
+    do_gogo. *)
+    (*
+    assert (H8 = H9).
+    { eapply gogo; eauto.
+    } *)
+
+    (*
+    subst.
+     *)
+    
+    
+    destruct_conjs.
+    exists x0.
+    split; eauto.
+    (*
+    +
+      eauto.
+      (*
+      eapply in_or_app.
+      eauto. *)
+    +
+      eauto. *)
+  - (* alseq case *)
+
+    df.
+    dosome_eq hi.
+    do_pair.
+    amsts.
+    df.
+    subst.
+    destruct t2.
+    +
+      destruct a eqn:aeq.
+      ++
+        doit.
+        
+        (*
+        dosome_eq hi.
+        dosome_eq hey.
+        subst.
+        repeat break_let.
+        do_pair.
+        dosome_eq hii.
+        subst.
+        do_pair.
+        dosome_eq hii.
+        dosome_eq hey.
+        subst.
+        repeat break_let.
+        do_pair.
+        dosome_eq hiii.
+        do_pair. *)
+        amsts.
+        (*
+        repeat dunit.
+        simpl.
+        simpl in hi.
+        simpl in Heqp2. *)
+        simpl in Heqp.
+        repeat break_let.
+        subst.
+        unfold ret in *.
+        do_pair.
+        do_pair.
+        measEventFacts.
+        evEventFacts.
+        invEvents.
+        (*
+        invc H0.
+        invc H. *)
+        +++
+          do_pl_immut.
+          cbn in Heqp1.
+          do_pair.
+
+          eapply IHt1 with (vmst:= {| st_ev := st_ev3; st_trace := st_trace3; st_pl := st_pl2; st_store := st_store3 |}) (new_vmst := {| st_ev := st_ev2; st_trace := st_trace4; st_pl := st_pl4; st_store := st_store4 |}).
+          eassumption.
+          tauto.
+          tauto.
+          tauto.
+          eassumption.
+          eassumption.
+          tauto.
+          econstructor.
+          eassumption.
+          econstructor.
+        +++
+          solve_by_inversion.
+      ++
+
+        doit.
+        (*
+
+        dosome_eq hi.
+        dosome_eq hey.
+        subst.
+        repeat break_let.
+        do_pair.
+        dosome_eq hii.
+        subst.
+        do_pair.
+        dosome_eq hii.
+        dosome_eq hey.
+        subst.
+        repeat break_let.
+        do_pair.
+        dosome_eq hiii.
+        do_pair. *)
+        amsts.
+        (*
+        repeat dunit.
+        simpl.
+        simpl in hi. *)
+        
+        (*
+        simpl in Heqp2.
+        repeat break_let.
+        subst.
+        unfold ret in *.
+        do_pair.
+        do_pair. *)
+        measEventFacts.
+        evEventFacts.
+        invEvents.
+        (*
+        invc H0.
+        invc H. *)
+        +++
+          do_pl_immut.
+          do_ba_st_const.
+          df.
+          dosome.
+          haaa.
+          
+          eapply IHt1 with (vmst:={| st_ev := st_ev3; st_trace := st_trace3; st_pl := st_pl2; st_store := st_store3 |}) (new_vmst:= {|
+                                                                                                                            st_ev := st_ev2;
+                                                                                                                            st_trace := st_trace1 ++ [umeas n3 0 n5 (n3 :: l)];
+                                                                                                                            st_pl := st_pl4;
+                                                                                                                            st_store := st_store4 |}).
+          eassumption.
+          tauto.
+          tauto.
+          tauto.
+          eassumption.
+          eassumption.
+          tauto.
+          econstructor.
+          eassumption.
+          econstructor.
+        +++
+          do_pl_immut.
+          do_ba_st_const.
+          invEvents.
+          (*
+          invc H5. *)
+          edestruct IHt2 with (vmst:={| st_ev := st_ev; st_trace := st_trace; st_pl := p; st_store := st_store |}) (new_vmst:={| st_ev := st_ev1; st_trace := st_trace1; st_pl := st_pl1; st_store := st_store1 |}).
+          eassumption.
+          tauto.
+          tauto.
+          tauto.
+          eassumption.
+          eassumption.
+          tauto.
+          econstructor.
+          econstructor.
+          reflexivity.
+          econstructor.
+          simpl in H.
+          destruct_conjs.
+          destruct r.
+          simpl in H1.
+          simpl.
+          exists x.
+          Print do_cumul2.
+          do_cumul.
+          subst.
+          split.
+          apply in_or_app.
+          eauto.
+          eauto.
+      ++
+        doit.
+        (*
+        dosome_eq hi.
+        dosome_eq hey.
+        subst.
+        repeat break_let.
+        do_pair.
+        do_pair.
+        dosome_eq hii.
+        subst.
+        do_pair.
+        dosome_eq hii.
+        do_pair.
+        dosome_eq hey.
+        subst.
+        repeat break_let.
+        dosome_eq hiii.
+        subst.
+        repeat break_let.
+        repeat 
+          do_pair.
+        dosome_eq hhhh.
+        subst.
+        do_pair. *)
+        unfold extractSig in *. simpl in Heqp7.
+        simpl in Heqp3.
+        destruct st_ev1; try solve_by_inversion.
+        unfold ret in *.
+        do_pair.
+        (*simpl in Heqp8. *)
+        break_match; try solve_by_inversion.
+        amsts.
+        do_ba_st_const.
+        do_pl_immut.
+        repeat dunit.
+        simpl.
+        
+        (*
+        simpl in Heqp2.
+        repeat break_let.
+        subst.
+        unfold ret in *.
+        do_pair.
+        do_pair. *)
+        measEventFacts.
+        evEventFacts.
+        invEvents.
+        (*
+        invc H0.
+        invc H. *)
+        +++
+          do_pl_immut.
+          do_ba_st_const.
+          (*
+          df.
+          dosome.
+          haaa. *)
+          do_pair.
+          df.
+          clear IHt2.
+          
+          eapply IHt1 with (vmst:={| st_ev := st_ev3; st_trace := st_trace3; st_pl := st_pl2; st_store := st_store3 |}) (new_vmst:= {|
+                                                                                                                            st_ev := e;
+                                                                                                                            st_trace := st_trace4 ++ [umeas n 0 n1 [encodeEv e; b]];
+                                                                                                                            st_pl := st_pl4;
+                                                                                                                            st_store := st_store4 |}).
+          eassumption.
+          tauto.
+          tauto.
+          tauto.
+          eassumption.
+          eassumption.
+          tauto.
+          econstructor.
+          eassumption.
+          econstructor.
+        +++
+          invEvents.
+
+    +
+      doit.
+      (*
+      dosome_eq hi.
+      dosome_eq hey.
+      subst.
+      repeat break_let.
+      do_pair.
+      dosome_eq hii.
+      subst.
+      do_pair.
+      dosome_eq hii.
+      dosome_eq hey.
+      subst.
+      repeat break_let.
+      do_pair.
+      dosome_eq hiii.
+      do_pair. *)
+      amsts.
+      (*
+      repeat dunit.
+      simpl.
+      simpl in hi. *)
+      simpl in Heqp.
+      repeat break_let.
+      subst.
+      unfold ret in *.
+      measEventFacts.
+      evEventFacts.
+      invEvents.
+      (*
+      invc H0.
+      invc H. *)
+      ++
+
+        clear IHt2.
+        df.
+        dohtac.
+        df.
+        do_pl_immut.
+        do_ba_st_const.
+        eapply IHt1 with (vmst:={| st_ev := st_ev3; st_trace := st_trace3; st_pl := st_pl2; st_store := st_store3 |}) (new_vmst:={| st_ev := st_ev2; st_trace := st_trace4; st_pl := st_pl4; st_store := st_store4 |}).
+        eassumption.
+        tauto.
+        tauto.
+
+        simpl.
+
+        
+
+
+        assert (st_ev4 = st_ev2).
+        { 
+          Check dood.
+          eapply dood with (vm_st0 := {| st_ev := st_ev4; st_trace := []; st_pl := n1; st_store := [] |}).
+          apply build_comp_at.
+          tauto.
+          tauto.
+          apply Heqp.
+          eassumption.
+          tauto.
+          tauto.
+        }
+        subst.
+        tauto.
+        eassumption.
+        eassumption.
+        tauto.
+        econstructor.
+        eassumption.
+        econstructor.
+      ++
+        do_pl_immut.
+        do_ba_st_const.
+        cbn in Heqp1.
+        repeat break_let.
+        df.
+        dohtac.
+        dosome.
+        do_pl_immut.
+        do_ba_st_const.
+        amsts.
+        df.
+        invEvents.
+        edestruct IHt2 with (vmst:={| st_ev := st_ev; st_trace := []; st_pl := n1; st_store := [] |}) (new_vmst:={| st_ev := toRemote (unanno t2) st_ev; st_trace := st_trace1; st_pl := st_pl1; st_store := st_store1 |}).
+        tauto.
+        tauto.
+
+        tauto.
+        tauto.
+        eassumption.
+        eassumption.
+        tauto.
+        econstructor.
+        apply evtsatt.
+        eassumption.
+        econstructor.
+
+        
+        destruct_conjs.
+        simpl in H1.
+        do_cumul.
+        subst.
+
+        exists x.
+        split.
+        +++
+          eapply in_or_app.
+          eauto.
+        +++
+          eauto.
+    +
+      doit.
+      (*
+
+      dosome_eq hi.
+      dosome_eq hey.
+      subst.
+      repeat break_let.
+      do_pair.
+      dosome_eq hii.
+      subst.
+      do_pair.
+      dosome_eq hii.
+      dosome_eq hey.
+      subst.
+      repeat break_let.
+      do_pair.
+      dosome_eq hiii.
+      do_pair. *)
+      amsts.
+      (*
+      repeat dunit.
+      simpl.
+      simpl in hi. *)
+
+      repeat break_let.
+      subst.
+      unfold ret in *.
+      measEventFacts.
+      evEventFacts.
+      invEvents.
+      (*
+      invc H0.
+      invc H. *)
+      ++
+
+        clear IHt2.
+        (*
+        df.
+        dohtac.
+        df. *)
+        do_pl_immut.
+        do_ba_st_const.
+        eapply IHt1 with (vmst:={| st_ev := st_ev3; st_trace := st_trace3; st_pl := st_pl2; st_store := st_store3 |}) (new_vmst:={| st_ev := st_ev2; st_trace := st_trace4; st_pl := st_pl4; st_store := st_store4 |}).
+        eassumption.
+        tauto.
+        tauto.
+
+
+        assert (st_ev = st_ev2).
+        {
+          Check dood.
+          eapply dood.
+          apply Heqp1.
+          tauto.
+          tauto.
+          eassumption.
+          eassumption.
+          tauto.
+          tauto.
+        }
+        subst.
+        tauto.
+        eassumption.
+        eassumption.
+        tauto.
+        econstructor.
+        eassumption.
+        econstructor.
+      ++
+        do_pl_immut.
+        do_ba_st_const.
+        (*
+        cbn in Heqp1.
+        repeat break_let.
+        df.
+        dohtac.
+        dosome.
+        do_pl_immut.
+        do_ba_st_const. 
+        amsts.
+        df. *)
+
+        (*invc H5. *)
+        edestruct IHt2 with (vmst:={| st_ev := st_ev; st_trace := st_trace; st_pl := st_pl2; st_store := st_store |}) (new_vmst:={| st_ev := st_ev1; st_trace := st_trace1; st_pl := st_pl1; st_store := st_store1 |}).
+        eassumption.
+        tauto.
+        tauto.
+        tauto.
+        eassumption.
+        eassumption.
+        tauto.
+        econstructor.
+        eassumption.
+        econstructor.
+        destruct_conjs.
+
+        do_cumul.
+        subst.
+        simpl in H.
+        exists x.
+        split.
+        +++
+          apply in_or_app.
+          eauto.
+        +++
+          eauto.
+          Unshelve.
+          exact (aasp (0,0) (ASPC 1 [])).
+          exact mtc.
+          eauto.
+          eauto.
+          exact (aasp (0,0) (ASPC 1 [])).
+          exact mtc.
+          eauto.
+          eauto.
+          exact (aasp (0,0) (ASPC 1 [])).
+          exact mtc.
+          eauto.
+          eauto.
+          exact (aasp (0,0) (ASPC 1 [])).
+          exact mtc.
+          eauto.
+          eauto.
+          exact (aasp (0,0) (ASPC 1 [])).
+          exact mtc.
+          eauto.
+          eauto.
+          exact (aasp (0,0) (ASPC 1 [])).
+          exact mtc.
+          eauto.
+          eauto.
+          exact (aasp (0,0) (ASPC 1 [])).
+          exact mtc.
+          eauto.
+          eauto.
+Defined.
